src/prelim/presetoid.lean
@@ -1,8 +1,15 @@
 import tactic .single .size
 
-/- WIP - the idea here is to clean up the definition of parallel in simple.lean using the fact 
-that it is transitive and symmetric -/
-universes u v w
+/-! 
+This file contains an API for a `presetoid`, which is a symmetric, transitive relation. This is
+essentially an equivalence relation, together with a 'kernel' of singletons that are not related
+to any elements, even themselves. This describes the 'parallel' relation in the edges of a graph, 
+or on the elements of the matroids; in both cases the kernel consists of loops. 
+
+The API contains basic lemmas and definitions for objects like equivalence classes, as well as 
+definitions of `simple` sets that are disjoint from the kernel and contain at most one element of
+each equivalence class. 
+-/
 
 open_locale classical 
 noncomputable theory 
@@ -14,28 +21,28 @@ structure presetoid (α : Type*) :=
 (rel_transitive : transitive rel)
 (rel_symmetric : symmetric rel)
 
-variables {α : Type*} {a b c : α} {s X : set α} (S : presetoid α) 
+variables {α : Type*} {a b c : α} {s X : set α} {S : presetoid α} 
 
 namespace presetoid 
 
-def kernel : set α := 
+def kernel (S : presetoid α): set α := 
   {x : α | ¬S.rel x x}
 
 lemma mem_kernel_iff : 
   a ∈ S.kernel ↔ ¬S.rel a a := 
 by simp [kernel]
 
-def cl (a : α) : set α :=
+def cl (S : presetoid α)(a : α) : set α :=
   { x : α | S.rel x a }
 
-def is_class (s : set α) : Prop := 
+def is_class (S : presetoid α)(s : set α) : Prop := 
   nonempty s ∧ ∃ a, s = S.cl a 
 
 lemma is_class_def {s : set α} : 
   S.is_class s ↔ (nonempty s ∧ ∃ a, s = S.cl a) :=
 iff.rfl 
 
-def classes : set (set α) := 
+def classes (S : presetoid α) : set (set α) := 
   { X | S.is_class X }
 
 lemma mem_classes_iff_is_class {X : set α} : 
@@ -52,14 +59,14 @@ S.rel_symmetric hab
 
 def rel_self_of_rel (ha : S.rel a b) : 
   S.rel a a := 
-S.trans ha (S.symm ha)
+trans ha (symm ha)
 
 @[simp] lemma cl_eq_empty_iff: 
   S.cl a = ∅ ↔ ¬S.rel a a := 
 begin
   rw [cl, sep_eq_empty_iff, ← not_iff_not],
   push_neg, 
-  exact ⟨λ h, let ⟨x,hx⟩ := h in S.rel_self_of_rel (S.symm hx), λ h, ⟨_,h⟩⟩, 
+  exact ⟨λ h, let ⟨x,hx⟩ := h in rel_self_of_rel (symm hx), λ h, ⟨_,h⟩⟩, 
 end
 
 @[simp] lemma cl_nonempty_iff: 
@@ -76,15 +83,15 @@ by rw [cl, mem_set_of_eq]
 
 lemma rel_of_mems_cl (ha : a ∈ S.cl c) (hb : b ∈ S.cl c) :
   S.rel a b :=
-S.trans (S.mem_cl_iff.mp ha) (S.symm (S.mem_cl_iff.mp hb))
+trans (mem_cl_iff.mp ha) (symm (mem_cl_iff.mp hb))
 
 lemma rel_self_of_mem_class {s : set α} (hs : S.is_class s) (ha : a ∈ s) :
   S.rel a a :=
-by {obtain ⟨hb, ⟨b,rfl⟩⟩ := hs, exact S.rel_self_of_rel (S.mem_cl_iff.mp ha), }
+by {obtain ⟨hb, ⟨b,rfl⟩⟩ := hs, exact rel_self_of_rel (mem_cl_iff.mp ha), }
 
 lemma rel_of_mems_class {s : set α} (hs : S.is_class s) (ha : a ∈ s) (hb : b ∈ s) :
   S.rel a b :=
-by {obtain ⟨-, x, rfl⟩ := hs, exact S.rel_of_mems_cl ha hb}
+by {obtain ⟨-, x, rfl⟩ := hs, exact rel_of_mems_cl ha hb}
 
 lemma mem_cl_self_iff: 
   a ∈ S.cl a ↔ S.rel a a := 
@@ -95,22 +102,22 @@ lemma is_class_iff_rep {X : set α} :
 begin
   refine ⟨λ h, _, λ h, _⟩,
   { obtain ⟨⟨b⟩, ⟨a,rfl⟩⟩ := h, 
-    exact ⟨a, S.rel_self_of_rel (S.mem_cl_iff.mp (S.symm b.2)), rfl⟩}, 
+    exact ⟨a, rel_self_of_rel (mem_cl_iff.mp (symm b.2)), rfl⟩}, 
   obtain ⟨a, ⟨ha,rfl⟩⟩ := h, 
-  exact ⟨⟨⟨a,S.mem_cl_iff.mpr ha⟩⟩,a,rfl⟩,
+  exact ⟨⟨⟨a,mem_cl_iff.mpr ha⟩⟩,a,rfl⟩,
 end
 
 lemma class_has_rep {X : set α} : 
   S.is_class X → (∃ a, (S.rel a a) ∧ X = S.cl a) :=
-S.is_class_iff_rep.mp 
+is_class_iff_rep.mp 
 
 lemma class_nonempty (hX : S.is_class X):
   X.nonempty := 
-by {obtain ⟨a,h₁,rfl⟩ := S.class_has_rep hX, exact ⟨a, S.mem_cl_self_iff.mp h₁⟩,  }
+by {obtain ⟨a,h₁,rfl⟩ := class_has_rep hX, exact ⟨a, mem_cl_self_iff.mp h₁⟩,  }
 
 lemma cl_is_class (ha : S.rel a a) :
   S.is_class (S.cl a) :=
-S.is_class_iff_rep.mpr ⟨a, ha, rfl⟩ 
+is_class_iff_rep.mpr ⟨a, ha, rfl⟩ 
 
 @[simp] lemma mem_classes_iff {X : set α} : 
   X ∈ S.classes ↔ (∃ a, (S.rel a a) ∧ X = S.cl a) :=
@@ -121,14 +128,14 @@ lemma cl_eq_cl_iff (ha : S.rel a a) :
 begin
   simp_rw [cl, ext_iff, mem_set_of_eq],
   refine ⟨λ h, by rwa ←h a, λ h, λ x, _⟩,
-  have := S.symm h, 
+  have := symm h, 
   split; {intro, transitivity; assumption}, 
 end
 
 def cl_eq_cl_of_rel (h : S.rel a b) : 
   S.cl a = S.cl b :=
 begin
-  have := S.symm h, 
+  have := symm h, 
   refine ext_iff.mpr (λ x, ⟨λ h, _, λ h, _⟩);
   {rw mem_cl_iff at *, transitivity; assumption}, 
 end 
@@ -136,18 +143,18 @@ end
 lemma class_eq_cl_mem (hs : S.is_class s) (ha : a ∈ s) :
   s = S.cl a := 
 begin
-  obtain ⟨b, hb, rfl⟩ := S.is_class_iff_rep.mp hs, 
-  exact (S.cl_eq_cl_of_rel (S.mem_cl_iff.mp ha)).symm, 
+  obtain ⟨b, hb, rfl⟩ := is_class_iff_rep.mp hs, 
+  exact (cl_eq_cl_of_rel (mem_cl_iff.mp ha)).symm, 
 end
 
-lemma eqv_classes_pairwise_disj : 
+lemma eqv_classes_pairwise_disj (S : presetoid α): 
   S.classes.pairwise_disjoint :=
 begin
   intros C₁ hC₁ C₂ hC₂ hC₁C₂, 
   refine disjoint_left.mpr (λ a ha₁ ha₂, hC₁C₂ _), 
-  obtain ⟨⟨x₁,h₁,rfl⟩,⟨x₂,h₂,rfl⟩⟩ := ⟨S.mem_classes_iff.mp hC₁, S.mem_classes_iff.mp hC₂⟩, 
+  obtain ⟨⟨x₁,h₁,rfl⟩,⟨x₂,h₂,rfl⟩⟩ := ⟨mem_classes_iff.mp hC₁, mem_classes_iff.mp hC₂⟩, 
   rw mem_cl_iff at ha₁ ha₂, 
-  rw (S.cl_eq_cl_iff h₁),  
+  rw (cl_eq_cl_iff h₁),  
   transitivity, symmetry, exact ha₁, assumption, 
 end
 
@@ -158,8 +165,8 @@ begin
   simp only [kernel, exists_prop, not_not, mem_set_of_eq, mem_classes_iff, mem_compl_eq],  
   split, 
   { rintro ⟨P, ⟨a, ha, rfl⟩, haP⟩, 
-    exact S.rel_self_of_rel (S.mem_cl_iff.mp haP), },
-  exact λ hx, ⟨S.cl x, ⟨_, hx,rfl⟩ , S.mem_cl_iff.mp hx⟩, 
+    exact rel_self_of_rel (mem_cl_iff.mp haP), },
+  exact λ hx, ⟨S.cl x, ⟨_, hx,rfl⟩ , mem_cl_iff.mp hx⟩, 
 end
 
 section simple
@@ -169,15 +176,61 @@ def is_simple_set (S : presetoid α) (X : set α) :=
   ∀ x y ∈ X, S.rel x y ↔ x = y 
 
 lemma simple_set_iff {S : presetoid α} {X : set α} : 
-  S.is_simple_set X ↔ disjoint X S.kernel ∧ ∀ P, S.is_class P → size (X ∩ P) ≤ 1 :=
+  S.is_simple_set X ↔ disjoint X S.kernel ∧ ∀ P, S.is_class P → (∀ e f ∈ X ∩ P, e = f) :=
 begin
-  refine ⟨λ h, _, λ h, _⟩, 
-  { by_contra hn, rw [not_and_distrib, not_disjoint_iff, not_forall] at hn, 
+  refine ⟨λ h, by_contra (λ hn, _), λ h, by_contra (λ hn, _)⟩, 
+  { rw [not_and_distrib, not_disjoint_iff, not_forall] at hn, 
     obtain (⟨x, hxX, hxK⟩ | ⟨P, hP⟩) := hn, 
     { rw mem_kernel_iff at hxK, exact hxK ((h x x hxX hxX).mpr rfl),  },
-    rw [not_imp] at hP, 
-    
-     }, 
+    push_neg at hP, 
+    obtain ⟨e,f,⟨heX, heP⟩,⟨hfX,hfP⟩,hef⟩ := hP.2,
+    exact hef ((h e f heX hfX).mp (rel_of_mems_class hP.1 heP hfP ))},
+  rw [is_simple_set] at hn,  
+  push_neg at hn, 
+
+  obtain ⟨e,f,he,hf,hef⟩ := hn, 
+  rw [not_iff] at hef, 
+  rcases em (e = f) with (rfl | hef'), 
+  { simp only [eq_self_iff_true, iff_true] at hef,
+    rw disjoint_right at h, 
+    exact (h.1 (mem_kernel_iff.mpr hef)) he},
+  rw [iff_false_intro hef', iff_false, not_not] at hef, 
+  have her := rel_self_of_rel hef, 
+  exact hef' (h.2 (S.cl e) (cl_is_class her) _ _ 
+    ⟨he, mem_cl_self_iff.mpr her⟩
+    ⟨hf, mem_cl_iff.mpr (symm hef)⟩ ), 
+end
+
+lemma simple_set_iff_of_fintype [fintype α] { X : set α }: 
+  S.is_simple_set X ↔ disjoint X S.kernel ∧ ∀ P, S.is_class P → size (X ∩ P) ≤ 1 :=
+by {conv in (_ ≤ _) {rw size_le_one_iff_mem_unique}, exact simple_set_iff} 
+
+/-- a presetoid is simple if its kernel is empty and its equivalence classes are singletons -/
+def is_simple (S : presetoid α) := 
+  S.is_simple_set univ 
+
+lemma simple_iff :
+  S.is_simple ↔ S.kernel = ∅ ∧ ∀ P, S.is_class P → size P = 1 :=
+begin
+  rw [is_simple, simple_set_iff], convert iff.rfl, simp, 
+  simp_rw [univ_inter], 
+  refine iff_iff_eq.mp ⟨λ h P hP e f he hf, eq_of_mems_size_one (h P hP) he hf, λ h P hP, _⟩, 
+  rw size_eq_one_iff_nonempty_unique_mem, 
+  exact ⟨class_nonempty hP, h P hP⟩,
+end
+
+lemma simple_iff_rel :
+  S.is_simple ↔ ∀ x y, S.rel x y ↔ x = y :=
+by {rw [is_simple, is_simple_set], finish}
+
+lemma simple_iff_cl :
+  S.is_simple ↔ ∀ x, S.cl x = {x} := 
+begin
+  simp_rw [simple_iff_rel, cl], 
+  refine ⟨λ h x, by {ext, finish}, λ h x y, _⟩, 
+  specialize h y, 
+  simp only [ext_iff, mem_singleton_iff, mem_set_of_eq] at h, 
+  apply h,   
 end
 
 end simple
@@ -186,13 +239,36 @@ section size
 
 variables [fintype α]
 
-lemma size_classes_le_type_size:
+lemma size_classes_le_type_size (S : presetoid α):
   size (S.classes) ≤ type_size α := 
 size_disjoint_collection_le_type_size 
-  (λ s hs, S.class_nonempty (S.mem_classes_iff_is_class.mpr hs))
+  (λ s hs, class_nonempty (mem_classes_iff_is_class.mpr hs))
   (S.eqv_classes_pairwise_disj)
 
---lemma size_classes_eq_type_size_i
+/- this proof is a nasty hack and should be improvable -/
+lemma size_classes_eq_type_size_iff_simple (S : presetoid α): 
+  size S.classes = type_size α ↔ S.is_simple :=
+begin
+  convert size_disjoint_collection_eq_type_size_iff 
+    (λ s hs, class_nonempty (mem_classes_iff_is_class.mpr hs))
+    (S.eqv_classes_pairwise_disj), 
+  rw [simple_iff, ← iff_iff_eq],  
+  congr' 2,
+  
+  refine iff_iff_eq.mp ⟨λ h, _, λ h, _⟩,  
+  { ext x, simp only [exists_prop, mem_univ, mem_set_of_eq, iff_true], 
+    refine ⟨S.cl x, mem_sep (mem_def.mp (nonempty.to_subtype ⟨x, mem_cl_self_iff.mpr _⟩)) _ , _⟩,  
+    { apply not_not.mp, rw [← mem_kernel_iff, h], apply not_mem_empty },
+    { exact ⟨x,rfl⟩},
+    { rw mem_cl_self_iff, apply not_not.mp, rw [← mem_kernel_iff, h], apply not_mem_empty }},
+  simp only [kernel, not_not, sep_eq_empty_iff], 
+  intro x, 
+  rw sUnion_eq_univ_iff at h, 
+  obtain ⟨X, h₁, h₂⟩ := h x, 
+  rw mem_def at h₁, 
+  obtain ⟨a, rfl⟩ := h₁.2, 
+  apply rel_of_mems_cl h₂ h₂,     
+end
 
 
 end size 
